Move spec of state to its own file

dm4good/State.v
@@ -5,7 +5,7 @@
 *)
 
 From Coq Require Import Utf8 RelationClasses.
-From PDM Require Import util guarded PURE PDM.
+From PDM Require Import util guarded PURE PDM StateSpec.
 
 Set Default Goal Selector "!".
 Set Printing Projections.
@@ -15,221 +15,106 @@ Section State.
 
   Context (state : Type).
 
-  (* Specification monad *)
+  (* Computation monad *)
 
-  Definition preᵂ := state → Prop.
-  Definition postᵂ A := state → A → Prop.
-
-  Definition W' A := postᵂ A → preᵂ.
-
-  Class Monotonous [A] (w : W' A) :=
-    ismono : ∀ (P Q : postᵂ A) s₀, (∀ s₁ x, P s₁ x → Q s₁ x) → w P s₀ → w Q s₀.
-
-  Definition W A := { w : W' A | Monotonous w }.
-
-  Definition as_wp [A] (w : W' A) `{h : Monotonous _ w} : W A :=
-    exist _ w h.
-
-  Definition retᵂ' [A] (x : A) : W' A :=
-    λ P s₀, P s₀ x.
-
-  Instance retᵂ_ismono [A] (x : A) : Monotonous (retᵂ' x).
-  Proof.
-    intros P Q s₀ hPQ h.
-    apply hPQ. apply h.
-  Qed.
-
-  Definition retᵂ [A] (x : A) : W A :=
-    as_wp (retᵂ' x).
-
-  Definition bindᵂ' [A B] (w : W A) (wf : A → W B) : W' B :=
-    λ P, val w (λ s₁ x, val (wf x) P s₁).
-
-  Instance bindᵂ_ismono [A B] (w : W A) (wf : A → W B) :
-    Monotonous (bindᵂ' w wf).
-  Proof.
-    destruct w as [w mw].
-    intros P Q s₀ hPQ h.
-    eapply mw. 2: exact h.
-    simpl. intros s₁ x hf.
-    destruct (wf x) as [wf' mwf].
-    eapply mwf. 2: exact hf.
-    assumption.
-  Qed.
-
-  Definition bindᵂ [A B] (w : W A) (wf : A → W B) : W B :=
-    as_wp (bindᵂ' w wf).
-
-  Definition reqᵂ' (p : Prop) : W' p :=
-    λ P s₀, ∃ (h : p), P s₀ h.
-
-  Instance reqᵂ_ismono : ∀ p, Monotonous (reqᵂ' p).
-  Proof.
-    intros p. intros P Q s₀ hPQ h.
-    destruct h as [hp h].
-    exists hp. apply hPQ. assumption.
-  Qed.
-
-  Definition reqᵂ (p : Prop) : W p :=
-    as_wp (reqᵂ' p).
-
-  Definition getᵂ' : W' state :=
-    λ P s, P s s.
-
-  Instance getᵂ_ismono : Monotonous getᵂ'.
-  Proof.
-    intros P Q s₀ hPQ h.
-    red. red in h.
-    apply hPQ. assumption.
-  Qed.
-
-  Definition getᵂ : W state :=
-    as_wp getᵂ'.
-
-  Definition putᵂ' (s : state) : W' unit :=
-    λ P s₀, P s tt.
-
-  Instance putᵂ_ismono : ∀ s, Monotonous (putᵂ' s).
-  Proof.
-    intros s. intros P Q s₀ hPQ h.
-    apply hPQ. assumption.
-  Qed.
-
-  Definition putᵂ (s : state) : W unit :=
-    as_wp (putᵂ' s).
-
-  Definition WSt : ReqMonad := {|
-    M := W ;
-    ret := retᵂ ;
-    bind := bindᵂ ;
-    req := reqᵂ
+  Definition M : ReqMonad := {|
+    M A := state → G (state * A) ;
+    ret A x := λ s₀, retᴳ (s₀, x) ;
+    bind A B c f := λ s₀, bindᴳ (c s₀) (λ '(s₁, x), f x s₁) ;
+    req p := λ s₀, reqᴳ p (λ h, (s₀, h))
   |}.
 
-  Definition wle [A] (w₀ w₁ : W A) : Prop :=
-    ∀ P s, val w₁ P s → val w₀ P s.
+  Definition getᴹ : M state :=
+    λ s, retᴳ (s, s).
 
-  Instance WOrder : Order WSt.
-  Proof.
-    exists wle.
-    intros A x y z h₁ h₂. intros P s₀ h.
-    apply h₁. apply h₂.
-    assumption.
-  Defined.
+  Definition putᴹ (s : state) : M unit :=
+    λ s₀, retᴳ (s, tt).
 
-  Instance hmono : MonoSpec WSt WOrder.
+  (* Effect observation *)
+
+  Definition θ' [A] (c : M A) : W' A :=
+    λ post s₀,
+      let '(p ; f) := c s₀ in
+      ∃ (h : p), let '(s₁, x) := f h in post s₁ x.
+
+  Instance θ_ismono : ∀ A (c : M A), Monotonous (θ' c).
   Proof.
-    constructor.
-    intros A B w w' wf wf' hw hwf.
-    intros P s₀ h.
-    do 3 red. do 3 red in h.
-    apply hw. destruct w' as [w' mw']. eapply mw'. 2: exact h.
-    simpl. intros s₁ x hf. apply hwf. assumption.
+    intros A c. intros P Q s₀ hPQ h.
+    red. red in h. destruct (c s₀) as [p f].
+    destruct h as [hp h]. exists hp.
+    destruct (f hp) as [s₁ x]. apply hPQ. assumption.
   Qed.
 
-  (* State transformer version *)
-  Section Passing.
+  Definition θ [A] (c : M A) : W A :=
+    as_wp (θ' c).
 
-    (* Computation monad *)
-
-    Definition M : ReqMonad := {|
-      M A := state → G (state * A) ;
-      ret A x := λ s₀, retᴳ (s₀, x) ;
-      bind A B c f := λ s₀, bindᴳ (c s₀) (λ '(s₁, x), f x s₁) ;
-      req p := λ s₀, reqᴳ p (λ h, (s₀, h))
-    |}.
-
-    Definition getᴹ : M state :=
-      λ s, retᴳ (s, s).
-
-    Definition putᴹ (s : state) : M unit :=
-      λ s₀, retᴳ (s, tt).
-
-    (* Effect observation *)
-
-    Definition θ' [A] (c : M A) : W' A :=
-      λ post s₀,
-        let '(p ; f) := c s₀ in
-        ∃ (h : p), let '(s₁, x) := f h in post s₁ x.
-
-    Instance θ_ismono : ∀ A (c : M A), Monotonous (θ' c).
-    Proof.
-      intros A c. intros P Q s₀ hPQ h.
-      red. red in h. destruct (c s₀) as [p f].
-      destruct h as [hp h]. exists hp.
-      destruct (f hp) as [s₁ x]. apply hPQ. assumption.
-    Qed.
-
-    Definition θ [A] (c : M A) : W A :=
-      as_wp (θ' c).
-
-    Instance θ_morph : LaxMorphism WOrder θ.
-    Proof.
-      constructor.
-      - intros A x. intros post s₀ h.
-        cbn. exists I. red in h. assumption.
-      - intros A B c f. intros post s₀ h.
-        unfold bind. simpl. unfold θ'.
-        unfold bind in h. simpl in h. unfold θ' in h.
-        destruct (c s₀) as [p c']. clear c.
-        destruct h as [hp h].
-        simpl.
-        unshelve eexists.
-        { exists hp. destruct (c' hp) as [s₁ x]. destruct (f x s₁).
-          simpl. destruct h. assumption.
-        }
-        simpl. destruct (c' hp) as [s₁ x]. destruct (f x s₁).
+  Instance θ_morph : LaxMorphism WStOrder θ.
+  Proof.
+    constructor.
+    - intros A x. intros post s₀ h.
+      cbn. exists I. red in h. assumption.
+    - intros A B c f. intros post s₀ h.
+      unfold bind. simpl. unfold θ'.
+      unfold bind in h. simpl in h. unfold θ' in h.
+      destruct (c s₀) as [p c']. clear c.
+      destruct h as [hp h].
+      simpl.
+      unshelve eexists.
+      { exists hp. destruct (c' hp) as [s₁ x]. destruct (f x s₁).
         simpl. destruct h. assumption.
-      - intro p. intros post s₀ h.
-        assumption.
-    Qed.
-
-    (* Partial Dijkstra monad *)
-
-    Definition D : DijkstraMonad WOrder :=
-      PDM.D M WSt WOrder hmono θ θ_morph.
-
-    (* Universe inconsistency *)
-    (* Definition getᴰ : D state getᵂ.
-    Proof.
-      exists getᴹ.
-      cbv. intros post s h. exists I. assumption.
-    Defined. *)
-
-    Definition putᴰ s : D unit (putᵂ s).
-    Proof.
-      exists (putᴹ s).
-      cbv. intros post s₀ h. exists I. assumption.
-    Defined.
-
-    (* Lift from PURE *)
-
-    Definition liftᵂ [A] (w : pure_wp A) : W A.
-    Proof.
-      exists (λ P s₀, val w (λ x, P s₀ x)).
-      intros P Q s₀ hPQ h.
-      destruct w as [w mw].
-      eapply mw. 2: exact h.
-      apply hPQ.
-    Defined.
-
-    Instance hlift : PureSpec WSt WOrder liftᵂ.
-    Proof.
-      constructor.
-      intros A w f.
-      intros P s h.
-      assert (hpre : val w (λ _, True)).
-      { unfold liftᵂ in h.
-        destruct w as [w hw].
-        eapply hw. 2: exact h.
-        auto.
       }
-      cbv. exists hpre.
-      pose proof (prf (f hpre)) as hf. simpl in hf.
-      apply hf in h. assumption.
-    Qed.
+      simpl. destruct (c' hp) as [s₁ x]. destruct (f x s₁).
+      simpl. destruct h. assumption.
+    - intro p. intros post s₀ h.
+      assumption.
+  Qed.
 
-    Check liftᴾ M WSt WOrder hmono θ θ_morph liftᵂ hlift.
+  (* Partial Dijkstra monad *)
 
-  End Passing.
+  Definition D : DijkstraMonad WStOrder :=
+    PDM.D M WSt _ WStMono θ θ_morph.
+
+  (* Universe inconsistency *)
+  (* Definition getᴰ : D state getᵂ.
+  Proof.
+    exists getᴹ.
+    cbv. intros post s h. exists I. assumption.
+  Defined. *)
+
+  Definition putᴰ s : D unit (putᵂ s).
+  Proof.
+    exists (putᴹ s).
+    cbv. intros post s₀ h. exists I. assumption.
+  Defined.
+
+  (* Lift from PURE *)
+
+  (* Universe problem again *)
+  (* Definition liftᵂ [A] (w : pure_wp A) : WSt A.
+  Proof.
+    exists (λ P s₀, val w (λ x, P s₀ x)).
+    intros P Q s₀ hPQ h.
+    destruct w as [w mw].
+    eapply mw. 2: exact h.
+    apply hPQ.
+  Defined.
+
+  Instance hlift : PureSpec WSt WOrder liftᵂ.
+  Proof.
+    constructor.
+    intros A w f.
+    intros P s h.
+    assert (hpre : val w (λ _, True)).
+    { unfold liftᵂ in h.
+      destruct w as [w hw].
+      eapply hw. 2: exact h.
+      auto.
+    }
+    cbv. exists hpre.
+    pose proof (prf (f hpre)) as hf. simpl in hf.
+    apply hf in h. assumption.
+  Qed.
+
+  Check liftᴾ M WSt WOrder hmono θ θ_morph liftᵂ hlift. *)
 
 End State.
