dm4good/StateSpec.v
@@ -1,0 +1,123 @@
+(* Specification monad for state *)
+
+From Coq Require Import Utf8 RelationClasses.
+From PDM Require Import util guarded PURE PDM.
+
+Set Default Goal Selector "!".
+Set Printing Projections.
+Set Universe Polymorphism.
+
+Section State.
+
+  Context {state : Type}.
+
+  Definition preᵂ := state → Prop.
+  Definition postᵂ A := state → A → Prop.
+
+  Definition W' A := postᵂ A → preᵂ.
+
+  Class Monotonous [A] (w : W' A) :=
+    ismono : ∀ (P Q : postᵂ A) s₀, (∀ s₁ x, P s₁ x → Q s₁ x) → w P s₀ → w Q s₀.
+
+  Definition W A := { w : W' A | Monotonous w }.
+
+  Definition as_wp [A] (w : W' A) `{h : Monotonous _ w} : W A :=
+    exist _ w h.
+
+  Definition retᵂ' [A] (x : A) : W' A :=
+    λ P s₀, P s₀ x.
+
+  Instance retᵂ_ismono [A] (x : A) : Monotonous (retᵂ' x).
+  Proof.
+    intros P Q s₀ hPQ h.
+    apply hPQ. apply h.
+  Qed.
+
+  Definition retᵂ [A] (x : A) : W A :=
+    as_wp (retᵂ' x).
+
+  Definition bindᵂ' [A B] (w : W A) (wf : A → W B) : W' B :=
+    λ P, val w (λ s₁ x, val (wf x) P s₁).
+
+  Instance bindᵂ_ismono [A B] (w : W A) (wf : A → W B) :
+    Monotonous (bindᵂ' w wf).
+  Proof.
+    destruct w as [w mw].
+    intros P Q s₀ hPQ h.
+    eapply mw. 2: exact h.
+    simpl. intros s₁ x hf.
+    destruct (wf x) as [wf' mwf].
+    eapply mwf. 2: exact hf.
+    assumption.
+  Qed.
+
+  Definition bindᵂ [A B] (w : W A) (wf : A → W B) : W B :=
+    as_wp (bindᵂ' w wf).
+
+  Definition reqᵂ' (p : Prop) : W' p :=
+    λ P s₀, ∃ (h : p), P s₀ h.
+
+  Instance reqᵂ_ismono : ∀ p, Monotonous (reqᵂ' p).
+  Proof.
+    intros p. intros P Q s₀ hPQ h.
+    destruct h as [hp h].
+    exists hp. apply hPQ. assumption.
+  Qed.
+
+  Definition reqᵂ (p : Prop) : W p :=
+    as_wp (reqᵂ' p).
+
+  Definition getᵂ' : W' state :=
+    λ P s, P s s.
+
+  Instance getᵂ_ismono : Monotonous getᵂ'.
+  Proof.
+    intros P Q s₀ hPQ h.
+    red. red in h.
+    apply hPQ. assumption.
+  Qed.
+
+  Definition getᵂ : W state :=
+    as_wp getᵂ'.
+
+  Definition putᵂ' (s : state) : W' unit :=
+    λ P s₀, P s tt.
+
+  Instance putᵂ_ismono : ∀ s, Monotonous (putᵂ' s).
+  Proof.
+    intros s. intros P Q s₀ hPQ h.
+    apply hPQ. assumption.
+  Qed.
+
+  Definition putᵂ (s : state) : W unit :=
+    as_wp (putᵂ' s).
+
+  Definition WSt : ReqMonad := {|
+    M := W ;
+    ret := retᵂ ;
+    bind := bindᵂ ;
+    req := reqᵂ
+  |}.
+
+  Definition wle [A] (w₀ w₁ : W A) : Prop :=
+    ∀ P s, val w₁ P s → val w₀ P s.
+
+  Instance WStOrder : Order WSt.
+  Proof.
+    exists wle.
+    intros A x y z h₁ h₂. intros P s₀ h.
+    apply h₁. apply h₂.
+    assumption.
+  Defined.
+
+  Instance WStMono : MonoSpec WSt WStOrder.
+  Proof.
+    constructor.
+    intros A B w w' wf wf' hw hwf.
+    intros P s₀ h.
+    do 3 red. do 3 red in h.
+    apply hw. destruct w' as [w' mw']. eapply mw'. 2: exact h.
+    simpl. intros s₁ x hf. apply hwf. assumption.
+  Qed.
+
+End State.
